# Gaussian Operators
The following definition Gaussian operators in terms of their 
Fourier property is made by [@bravyi2005classical].

::: {.definition #gaussianDef name="Gaussian operator"}
An operator $A\in \Cl_{2n}$ with $\tr(A)\neq 0$ is affine Gaussian if 
\[ 
    X(\theta) = C\exp\left(\df 1 2 \theta^T M\theta + d^T\theta\right)
\] 
for some antisymmetric $(M_{jk})\in \mbb C^{2n\times 2n}$ and 
$d\in \mbb C^{2n}$. It is (even) Gaussian if $d$ vanishes, which is 
equivalent to $X(\theta)$ being homogeneously even. 
Traceless Gaussians are defined as limits.
Two special cases

- Affine Gaussian hermitian operator: 
\[ 
    H(\theta) = C\exp\left(\df i 2 \theta^T h\theta + d^T\theta\right), 
    \quad (h_{jk})\in \mfk{so}(2n, \mbb R), \quad (d_j)\in \mbb R^{2n}
\] 
- Affine Gaussian unitary: 
\[ 
    U(\theta) = C\exp\left(\df 1 2 \theta^T u\theta + id^T\theta\right), 
    \quad (u_{jk})\in \mfk{so}(2n, \mbb R), \quad (d_j)\in \mbb R^{2n}
\] 
:::
Unlike in traditional statistics, fermionic Gaussians with zero mean 
is the norm rather than exception for most existing research. This is 
partly due to the boson-fermion superselection rule. 
We focus on even Gaussians first then extend known results, as possible, 
to affine Gaussians. 

## Even Gaussian
### Even Gaussian operators

### Characterization
::: {.theorem #evenGaussianEffect
name="effect of Gaussian unitaries"}
Consider a Gaussian unitary 
\[ 
    U = \exp\left(\df 1 2 \gamma^T h \gamma\right), \quad h_{jk}=-h_{kj}\in \mbb R 
\] 
Then it affects rotation of the majorana operators 
\[ 
    U \gamma_j U^\dag = R_{jk}\gamma_k, \quad R = e^{2h}
\] 
:::
_Proof:_ Using standard Lie theory technique, define $\gamma_j=\theta(0)$ and 
\[ 
    \theta(t) = U(t) \theta(0) U(t)^\dag
    = \tilde \gamma_j(t)\gamma_j, \quad U(t) = \exp\left(\df t 2 \gamma^T h \gamma \right)
\] 
Differentiation yields 
\[ 
    \pd t \theta(t) = 
    \left[\df 1 2 \gamma^T h \gamma, \theta(t) \right]
\] 
The key here is the commutator bracket. 
Using $[\gamma_a\gamma_b, \gamma_a]=-2\gamma_b$ we obtain 
\begin{align}
    \pd t \theta(t) 
    &= \df 1 2 \sum_{a, b, j} \tilde \gamma_j(t)h_{ab}[\gamma_a\gamma_b, \gamma_j]
    = \df 1 2 \sum_{b, j} \tilde \gamma_j(t)h_{jb}[\gamma_j\gamma_b, \gamma_j]
    + \df 1 2 \sum_{a, j} \tilde \gamma_j(t)h_{aj}[\gamma_a\gamma_j, \gamma_j] \\ 
    &= \sum_{j, b} -2 h_{jb} \tilde \gamma_j(t) \gamma_b
    = \sum_b \pd t \tilde \gamma_b(t)\gamma_b  \\ 
    \pd t \tilde \gamma_b(t) &= -2 h_{jb} \gamma_j(t) = 2h_{bj}\gamma_j(t)
\end{align}
The solution to this differential equation is 
\[ 
    \tilde \gamma(t) = R(t)\tilde \gamma(0), \quad R(t) = e^{2h} \in SO(2n)
\] 
It follows that $(UXU^\dag)(\theta) = X(R\theta)$. 

::: {.theorem #unifiedGaussian
name="characterization of Gaussian states"}
The following three characterizations of Gaussian states $\rho$ 
are equivalent. 

- $\rho(\theta) = 2^{-n} \exp(i \theta^T M \theta/2)$. 
- $\rho(\theta) = U(|0\ra \la 0|)^{\otimes n}U^\dag$, for some 
    Gaussian unitary $U$. 
- $\rho = e^{H}/\tr(e^H)$ for some $H$ which is homogeneously quadratic in 
    majorana operators. Pure states are defined in the limit 
    $H\mapsto \lim_{t\to \infty} tH$. 
:::
 

### Fourier perspective 
Bravyi's work [@bravyi2004lagrangian] provides many important 
results about Gaussian operators and maps from the Fourier perspective.

::: {.theorem #fourierEvenGaussianCharacterization 
name="fourier characterization of Gaussian operators"}

An operator $X\in \Cl_{2n}$ is Gaussian iff it is even and satisfies 
\[ 
    [\hat \Lambda, X\otimes X]=0, \quad \hat \Lambda = \gamma_a\otimes \gamma_a
\] 
:::

_Proof:_ We first derive the adjoint action of $\hat \Lambda$ in fourier space 
\@ref(lem:adjointLambda). 
The two directions \@ref(lem:fourierEvenGaussianfwd), 
\@ref(lem:fourierEvenGaussianbwd) follow. 

::: {.lemma #adjointLambda}
Consider the following differential operator 
$\Delta_a:\Gr_{2n}\otimes \Gr_{2n}\to \Gr_{2n}\otimes \Gr_{2n}$. 
\[ 
    \Delta_a = 2(\theta_a\otimes \pd a + \pd a \otimes \theta_a)
\] 
For any $Y, Z\in \Cl_{2n}$ having the same parity 
\[  
    [\gamma_a\otimes \gamma_a, Y\otimes Z](\theta) = \Delta_a[Y(\theta)\otimes Z(\theta)]
\] 
:::
_Proof:_ Take $Y, Z$ to be monomials $\gamma_J, \gamma_K$. 
If neither $J, K$ contains $a$ then both sides vanish. 
If both $J, K$ contains $a$, then the LHS vanishes by commutation, 
and both terms of the RHS are annihilated by $\theta_a$. 
If only $J$ contains $a$, then $\gamma_a\otimes \gamma_a$ anticommutes with 
$\gamma_J\otimes \gamma_K$ since $J$ contains one less factor than $K$ for $\gamma_a$ 
to commute across, then 
\[ 
    [\gamma_a\otimes \gamma_a, \gamma_J\otimes \gamma_K] 
    = 2 \gamma_a \gamma_J \otimes \gamma_a \gamma_K 
\] 
On the right hand side, only the second term in $\Delta_a$ survives, with 
\[ 
    2 (\pd a \otimes \theta_a) \theta_J \otimes \theta_K 
\] 
The two coefficients are seen to be equal: commuting $\pd a$ (resp. $\gamma_a$) 
across $\gamma_J$ (resp. $\theta_J$) takes the same number of swaps. 

::: {.lemma #fourierEvenGaussianfwd}

Given a Gaussian operator $X(\theta)=\exp(i\theta^TM\theta/2)$
\[ 
    \sum_a \Delta_a[X(\theta)\otimes X(\theta)]=0\implies [\Lambda, X\otimes X] = 0 
\] 
The traceless case follows by continuity. 
:::

_Proof:_ First compute $\pd a X = i M_{ab}\theta_b X$. This is not at all 
apparant as it seems, the exponential property arises from the power rule 
$\pd x x^n = nx^{n-1}$, which is only true in Grassmann calculus if 
$x$ (in this case $iM_{ab}\theta^TM\theta/2$) is even. Then 
\begin{equation}\begin{aligned}
\left[\hat \Lambda, X\otimes X\right](\theta)
&= 2\sum_a \left(\theta_a \otimes \pd a + \pd a \otimes \theta_a \right)
\exp\left(\df i 2 \theta^T M \theta\right)^{\otimes 2} \\ 
&= 2\sum_{a, b} \theta_a X \otimes iM_{ab} \theta_b X + iM_{ab} \theta_b X \otimes \theta_a X  \\ 
&= 2 i \sum_{a, b} M_{ab} (\theta_a \otimes \theta_b) (X\otimes X) = 0
\end{aligned}\end{equation}

::: {.lemma #fourierEvenGaussianbwd}
Suppose $X\in \Cl_{2n}$ is even with $\sum \Delta_a [X(\theta)\otimes X(\theta)]=0$, 
then $X$ is Gaussian. 
:::

_Proof:_ We provide the proof for non-vanishing trace case. 
Pin down the degree expansion of $X(\theta)$ 
\[ 
    X(\theta) = C + \df{iC}{2} M_{ab}\theta_a\theta_b + O(\theta^4) 
    \iff X(\theta) = C \exp\left(\df{i}{2} M_{ab}\theta_a\theta_b + \cdots\right)
\] 
Apply $1\otimes \pd b$ to the equation of interest, yielding 
\begin{aligned}
    0 &= (1\otimes \pd b) \sum_a (\theta_a X \otimes \pd a X + \pd a X\otimes \theta_a X) \\ 
    &= \sum_a \theta_aX \otimes \pd {ba}^2 X + \pd a X \otimes (\delta_{ab}X - \theta_a \pd b X) \\ 
    &= \pd b X \otimes X + \sum_a \theta_aX \otimes \pd {ba}^2 X - \pd a X \otimes \theta_a \pd b X \\
\end{aligned}
Consider the weaker equation where we only look at the linear term in the second 
tensor component, then the last term above vanishes due to $\theta_a$ 
and the equation simplifies to 
\begin{aligned}
    0 &= \pd b X \otimes C + \sum_a \theta_aX \otimes \df{iC}{2}M_{ab} \implies 
    0 = \pd b X + \df i 2 \sum_a M_{ab} \theta_a X 
\end{aligned}
This suffices to show that $X$ must be Gaussian.


### Even Gaussian linear maps
::: {.definition #gaussianMapDef name="Gaussian linear map"}
A linear map $\mca E:\Cl_{2n}\to \Cl_{2n}$ is Gaussian if 
\[ 
    \mca E(X)(\theta) = C\int D\eta\, D\mu\, 
    \exp \left[S(\theta, \eta) + i \eta^T \mu\right] X(\mu), \quad 
    S(\theta, \eta) = \df i 2 \begin{pmatrix}
        \theta \\ \eta
    \end{pmatrix} ^T \begin{pmatrix}
        A & B \\ -B^T & D 
    \end{pmatrix} \begin{pmatrix}
        \theta \\ \eta
    \end{pmatrix}
    (\#eq:gaussianLinearMap)
\] 
Here $A, D$ are antisymmetric and $B$ arbitrary. All values are complex. 
:::

::: {.example #identityExample name="identity map"}
Recalling the Grassmann dirac delta \@ref(def:diracDelta). 
\[ 
    X(\theta) = \int D\eta\, D\mu\, \exp(i\theta^T\eta + i\eta^T\mu) X(\mu) 
    \implies S = \begin{pmatrix}
        0 & I \\ -I & 0
    \end{pmatrix}
\] 
:::

::: {.proposition}
Gaussian linear maps are parity-preserving. 
:::
_Proof:_ Consider the automorphism $\overline{(\cdot)}$ 
such that $\overline X(\theta) = X(-\theta)$. It suffices to prove that 
\[ 
    \overline{\mca E(X)} = \mca E(\overline X)
\] 
Here $\overline{\mca E(X)}(\theta)$ is equivalent to replacing 
$\theta\mapsto -\theta$ in \@ref(eq:gaussianLinearMap), while $\mca E(\overline X)(\theta)$ 
is equivalent to replacing $\mu\mapsto -\mu$. 
They yield the same expression upon substitution by virtue of $S(\theta, -\eta) = S(-\theta, \eta)$ 
and $D(-\mu) = D\mu, D(-\eta) = D\eta$. 


::: {.proposition}
Gaussian linear maps map Gaussian operators into Gausian operators. 
:::
_Proof:_ Since $\mca E$ is parity preserving, it suffices to apply 
\@ref(thm:fourierEvenGaussianCharacterization) on $\mca E(X)$, for $X$ Gaussian. 
Note the following identity 
\begin{equation}
    \sum_a (\theta_a\otimes \pd {\theta_a} + \pd {\theta_a}\otimes \theta_a) 
        (e^{i\theta^TB\eta})^{\otimes 2}
    = -\sum_a (\eta_a\otimes \pd {\eta_a} + \pd {\eta_a}\otimes \eta_a) 
        (e^{i\theta^TB\eta})^{\otimes 2}
    (\#eq:convenientIdentity)
\end{equation}
We also need the Leibniz rule \@ref(prp:leibniz) and integration 
by part formula \@ref(prp:integrationByPart). Rewrite \@ref(eq:gaussianLinearMap) 
using an auxillary polynomial $f(\eta)$ 
\[ 
    \mca E(X)(\theta) = C\int D\eta\, 
    \exp \left[S(\theta, \eta)\right] f(\eta), \quad 
    f(\eta) = \int D\mu\, e^{i\eta^T\mu} X(\mu)
\] 
One can show that $f(\eta)$ is even. One can go on to show that 
\[ 
    \Lambda_{\mrm{ad}} \, \mca E(X)\otimes \mca E(X) 
    = \mca E\otimes \mca E(\Lambda_{\mrm{ad}}\, X\otimes X) = 0
\] 

::: {.proposition name="effect of Gaussian linear maps"}
Let $X$ be a Gaussian operator with correlation $M$ and pre-exponential 
factor $C$, then $\mca E(X)$ as defined in \@ref(eq:gaussianLinearMap) 
has correlation matrix 
\[ 
    \mca E(M) = B(M^{-1}+D)^{-1}B^T + A 
\] 
The pre-exponential factor is 
\begin{aligned}
    \tr\, \mca E(X) &= C (-1)^n \Pf(M)\Pf(M^{-1}+D)\tr(X) \\ 
    \tr[\mca E(X)]^2 &= C^2 \det (I+MD)\tr(X)^2
\end{aligned}
:::

_Proof:_ 

## Lie algebra embedding
Results from [@knill2001fermionic] provide the mathematical 
link between even and affine Gaussians. 

::: {.definition #gaussianLie name="Gaussian Lie groups and algebras"}
Fixing $n$ fermionic modes

- Let $\mca L_1, \mca L_2$ denote the linear and quadratic polynomials in $2n$ 
    majorana operators, respectively. 
- Let $\mca L_2'$ denote quadratic monomials. 
    Note that $\dim \mca L_2=2n^2 + n + 1, \dim \mca L_2'=2n^2-n$. 
- Let $\mca L_2^*$ denote the quadratic polynomials without constant terms, so 
    $\dim \mca L_2^*=2n^2+n$. 
:::

::: {.theorem #evenReduction name="even Gaussian algebra reduction"}
the affine Gaussian algebra $\mca L_2^*$ is isomorphic to a subalgebra 
of the even Gaussian algebra $\mca L_2'$ on one more mode.
:::

_Proof:_ Let the new mode append majorana operators $\gamma_{2n+1}, \gamma_{2n+2}$. 
Consider $\iota:\mca L_2^*\to \mca L_2'$ defined by 
\[ 
    \iota(\gamma_j) = i \gamma_j \gamma_{2n+1}, \quad 
    \iota(\gamma_j\gamma_k) = \gamma_j\gamma_k
\] 
In short, it appends $i\gamma_{2n+1}$ to linear terms and 
leaves quadratic terms unchanged. This is manifestly and injection, to 
demonstrate embedding it then suffices to show that 
$\iota\, [a, b] = [\iota\, a, \iota\, b]$. Consider the following representative 
cases with nonvanishing brackets
\begin{aligned}
    \iota\, [\gamma_1, \gamma_2] &= \iota(2\gamma_1\gamma_2) = 2\gamma_1\gamma_2 \\ 
    [\iota\, \gamma_1, \iota\, \gamma_2] 
    &= [i\gamma_1\gamma_{2n+1}, i\gamma_2\gamma_{2n+1}] = 2\gamma_1\gamma_2 \\ 
    \iota[\gamma_1, \gamma_1\gamma_2] 
    &= \iota(2\gamma_2) = 2i\gamma_2\gamma_{2n+1} \\ 
    [\iota\, \gamma_1, \iota\, \gamma_1\gamma_2] 
    &= [i\gamma_1\gamma_{2n+1}, \gamma_1\gamma_2] = 2i\gamma_2\gamma_{2n+1}
\end{aligned}

::: {.corollary #evenReductionCor name="even Gaussian unitary reduction"}
The affine Gaussian unitary group on $n$ fermionic modes is isomorphic to 
a subgroup of the even Gaussian unitary group on $n+1$ fermionic modes. 
:::

## Affine Gaussian